# Sorting: Homework 2

1. <a name="point1"></a> *Generalize the $\mathtt{SELECT}$ algorithm to deal also with repeated values and prove that it still belongs to $O(n)$.*
2. *Download the latest version of the code from*
                                                                                                                   *https://github.com/albertocasagrande/AD_sorting*
*and*
                                     - *Implement the $\texttt{SELECT}$ algorithm of Ex. [1](#point1).*
                                     - *Implement a variant of the $\texttt{QUICK SORT}$ algorithm using above-mentioned $\texttt{SELECT}$ to identify the best pivot for partitioning.*
                                     - *Draw a curve to represent the relation between the input size and the execution-time of the two variants of $\texttt{QUICK SORT}$ (i.e, those of Ex. 2 and Ex. 1 of [this file](#homework_03_01_SOLVED.md)) and discuss about their complexities.*                                   
3. *(Ex. 9.3-1 in [[1]](#ref1)) In the algorithm $\texttt{SELECT}$, the input elements are divided into chunks of $5$. Will the algorithm work in linear time if they are divided into chunks of $7$? What about chunks of $3$?*
4. *(Ex. 9.3-5 in [[1]](#ref1) Suppose that you have a "black-box" worst-case linear-time subroutine to get the position in $A$ of the value that would be in position $n/2$ if $A$ was sorted. Give a simple, linear-time algorithm that solves the selection problem for an arbitrary position $i$.*
5. *Solve the following recursive equations by using both the recursion tree and the substitution method:*
   - $T_1(n) = 2 * T_1(n/2) + O(n)$
   
     Using the **recursion tree**, we have that, choosing $cn$ as representative for $O(n)$
     $$
     \begin{align*}
     T_1(n) &= 2 * T_1(n/2) + O(n) \\
     &\le 2 * T_1(n/2) + cn \\
     &\le 2 * (2 * T_1(n/4) + cn/2) + cn \\
     &= 4 * T_1(n/4) + 2cn \\
     &\le 4 *(2 * T_1(n/8) + cn/4) + 2cn \\
     &= 8 * T_1(n/8) + 3cn\\
     &\le \ldots \\
     &\le 2^{\log_2 n} T_1(0) + \log_2 n * cn \\
     &= n * 0 + c n \log_2 n \in O(n \log n)
     \end{align*}
     $$
     or directly
     $$
     T_1(n) = 2 * T_1(n/2) + O(n) \le \sum_{i=0}^{\log_2 n} 2^i c \frac n{2^i} = \sum_{i=0}^{\log_2 n} cn = cn \sum_{i=0}^{\log_2 n} 1 = cn \log_2 n \in O(n \log n)
     \nonumber
     $$
     Using the **substitution method**, we guess that $T_1(n) \in O(n \log n)$. We select a representative for $O(n \log n)$ and $O(n)$, e.g. $cn \log n$ and $c' n$. We assume that $\forall m < n, \; T_1(m) \le cm \log m$. If this is the case,
     $$
     \begin{align*}
     T_1(n) &= 2 * T_1(n/2) + c'n \\
     &\le 2 * c n/2 \log(n/2) + c' n \\
     &= cn (\log n - \log 2) + c'n \\
     &= cn \log n - cn \log 2 + c'n \\
     &= cn \log n - cn + c'n
     \end{align*}
     $$
     if $c' n - cn \le 0 \Longleftrightarrow c' n \le cn \Longleftrightarrow c \ge c'$ then $T_1(n) \le c n \log n$. Thus we have proved by induction that $\forall n \in \mathbb{N}, \; T_1(n) \le c n \log n$ for a proper $c$. So $T_1(n) \in O(n \log n)$.
     
   - $T_2(n) = T_2(\lceil n/2 \rceil) + T_2(\lfloor n/2 \rfloor) + \Theta(1)$
   
     Using the **recursion tree**, we have that, choosing $c$ as representative for $O(1)$:
     $$
     \begin{align*}
     T_2(n) &= T_2(\lceil n/2 \rceil) + T_2(\lfloor n/2 \rfloor) + \Theta(1) \\
     &= T_2(\lceil n/2 \rceil) + T_2(\lfloor n/2 \rfloor) + c \\
     &= (T_2(\lceil \lceil n/2 \rceil/2 \rceil) + T_2(\lfloor \lceil n/2 \rceil/2 \rfloor) + c) + (T_2(\lceil \lfloor n/2 \rfloor/2 \rceil) + T_2(\lfloor \lfloor n/2 \rfloor/2 \rfloor) + c) + c
     \end{align*}
     $$
     if $n$ is even then we can simply remove the floor and ceiling functions, if $n$ is odd instead, so if $n = m+1$ with $m$ even, we have that
     $$
     \left\lceil \frac{\lfloor n/2 \rfloor}2 \right\rceil = \left\lceil \left(\frac m2 +1 \right)/2 \right\rceil = \left\lceil \frac m4 + \frac12 \right\rceil = \left\lceil \frac m4 + \frac14 \right\rceil = \left\lceil \frac{m+1}4 \right\rceil = \left\lceil \frac n4 \right\rceil \\
     \left\lfloor \frac{\lceil n/2 \rceil}2 \right\rfloor = \left\lfloor \left(\frac m2 +1 \right)/2 \right\rfloor = \left\lfloor \frac m4 + \frac12 \right\rfloor = \left\lceil \frac m4 \right\rceil = \left\lceil \frac n4 \right\rceil \\
     \left\lceil \frac{\lfloor n/2 \rfloor}2 \right\rceil = \left\lceil \left(\frac m2 \right)/2 \right\rceil =  \left\lceil \frac m4 \right\rceil = \left\lceil \frac m4 + \frac 14 \right\rceil = \left\lceil \frac{m+1}4 \right\rceil = \left\lceil \frac n4 \right\rceil \\
     \left\lfloor \frac{\lfloor n/2 \rfloor}2 \right\rfloor = \left\lfloor \left(\frac m2 \right)/2 \right\rfloor =  \left\lfloor \frac m4 \right\rfloor = \left\lfloor \frac m4 + \frac 14 \right\rfloor = \left\lfloor \frac{m+1}4 \right\rfloor = \left\lfloor \frac n4 \right\rfloor
     \nonumber
     $$
     so it follows that
     $$
     \begin{align*}
     T_2(n) &= T_2(\lceil n/4 \rceil) + T_2(\lceil n/4 \rceil) + T_2(\lceil n/4 \rceil) + T_2(\lfloor n/4 \rfloor) + 3c \\
     &= 3T_2(\lceil n/4 \rceil) + T_2(\lfloor n/4 \rfloor) + 3c \\
     &= 3(T_2(\lceil \lceil n/4 \rceil/2 \rceil) + T_2(\lfloor \lceil n/4 \rceil/2 \rfloor) + c) + (T_2(\lceil \lfloor n/4 \rfloor/2 \rceil) + T_2(\lfloor \lfloor n/4 \rfloor/2 \rfloor) + c) + 3c \\
     &= 3(T_2(\lceil n/8 \rceil) + T_2(\lceil n/8 \rceil) + c) + (T_2(\lceil n/8 \rceil) + T_2(\lfloor n/8 \rfloor) + c) + 3c \\
     &= 3T_2(\lceil n/8 \rceil) + 3T_2(\lceil n/8 \rceil) + 3c + T_2(\lceil n/8 \rceil) + T_2(\lfloor n/8 \rfloor) + c + 3c \\
     &= 7T_2(\lceil n/8 \rceil) + T_2(\lfloor n/8 \rfloor) + 7c \\
     &= \ldots \\
     &= (2^{\log_2 n} - 1) T(0) + T(0) + c(2^{\log_2 n} - 1) \\
     &= 0 + 0 + c(n-1) \in O(n)
     \end{align*}
     $$
     Or alternatively
   
     We have that the tree is complete up to the length of the shortest branch (which is the rightmost) â†’ it is the shortest branch, while the left one is the longest.
   
     For sure there exist a power of $2$ between $n$ and $2n$, and between $\frac n2$ and $n$, so the length of the recursion tree is $\le \log_2(2n)$ and $\ge \log_2(\frac n2)$.
     $$
     \begin{align*}
     T_2(n) &\ge \sum_{i=0}^{\log_2(\frac n2)} c 2^i = c \sum_{i=0}^{\log_2(\frac n2)} 2^i = c \cdot \frac{2^{\log_2(\frac n2) + 1} - 1}{2 - 1} = c \cdot \left( 2 \left( \frac n2 \right) - 1\right) = c(n-1) = cn - c \in \Omega(n) \\
     
     T_2(n) &\le \sum_{i=0}^{\log_2(2n)} c' 2^i =  c' \sum_{i=0}^{\log_2(2n)} 2^i = c' \cdot \frac{2^{\log_2(2n) + 1} - 1}{2 - 1} = c' \cdot \left( 2(2n) - 1\right) = c'(4n-1) = 4c'n - c' \in O(n)
     \end{align*}
     $$
     So we have that $T_2(n) \in \Theta(n)$.
   
     Using the **substitution method**, we guess that $T_2 \in O(n)$ and we select the function $cn$ as representative, and we select $c'$ as representative of $\Theta(1)$. Inductive assumption: we assume that $\forall m < n, \; T_2(m) \le cm$. We want to prove that $\forall n, \; T_2(n) \le cn$. If this is the case we have that
     $$
     \begin{align*}
     T_2(n) &= T_2(\lceil n/2 \rceil) + T_2(\lfloor n/2 \rfloor) + \Theta(1) \\
     &\le T_2(\lceil n/2 \rceil) + T_2(\lfloor n/2 \rfloor) + c' \\
     &\le c \lceil n/2 \rceil + c \lfloor n/2 \rfloor + c' \\
     &\le c(\lceil n/2 \rceil + \lfloor n/2 \rfloor) + c' \\
     &\le cn + c'
     \end{align*}
     $$
     But this is **not** what we wanted to prove, we cannot conclude anything! This doesn't prove $T_2 \in O(n)$ because $cn + c' \not\le cn$: but we are not able to prove it for a term of lower order. The problem is that we selected the wrong representative for $O(n)$, let us choose $cn - d \in O(n)$. Inductive assumption: we assume that $\forall m < n, \; T_2(m) \le cm - d$. We want to prove that $\forall n, \; T_2(n) \le cn - d$.
     $$
     \begin{align*}
     T_2(n) &= T_2(\lceil n/2 \rceil) + T_2(\lfloor n/2 \rfloor) + \Theta(1) \\
     &\le T_2(\lceil n/2 \rceil) + T_2(\lfloor n/2 \rfloor) + c' \\
     &\le c \lceil n/2 \rceil - d + c \lfloor n/2 \rfloor - d + c' \\
     &\le c(\lceil n/2 \rceil + \lfloor n/2 \rfloor) - 2d + c' \\
     &\le cn -2d + c'
     \end{align*}
     $$
     If $c' - d \le 0 \Longleftrightarrow c' \le d$, then $T_2(n) \le cn - d$. Thus we have proved by induction that $\forall n \in \mathbb{N}$, $T_2(n) \le c n - d$ for proper $c$ and $d$. So $T_2(n) \in O(n)$.
   
     Now we want to prove that $T_2(n) \in \Omega(n)$. We select the representative $cn \in \Omega(n)$ and the representative $c' \in \Theta(1)$. Inductive assumption: we assume that $\forall m < n, \; T_2(m) \ge cm$. We want to prove that $\forall n, \; T_2(n) \ge cn$.
     $$
     \begin{align*}
     T_2(n) &= T_2(\lceil n/2 \rceil) + T_2(\lfloor n/2 \rfloor) + \Theta(1) \\
     &\ge T_2(\lceil n/2 \rceil) + T_2(\lfloor n/2 \rfloor) + c' \\
     &\ge c \lceil n/2 \rceil + c \lfloor n/2 \rfloor + c' \\
     &\ge c(\lceil n/2 \rceil + \lfloor n/2 \rfloor) + c' \\
     &\ge cn + c' \\
     &\ge cn
     \end{align*}
     $$
     Thus we have that $T_2(n) \ge cn$, so we have proved by induction that $\forall n \in \mathbb{N}$, $T_2(n) \ge c n$ for a proper $c$. Then $T_2(n) \in \Omega(n)$. Therefore we have proved that $T_2(n) \in \Theta(n)$.
   
     By using substitution method, you can prove that $T_2(n) \in O(n^2)$. This is not wrong, because $O(n) \subseteq O(n^2)$, however this is a curse complexity bound.
   
   - $T(n) = T\left( \frac 15 n \right) + T \left(\frac34 n \right) + \Theta(n)$
   
     This equation is weird because it is totally unbalanced! All the branches are different in length! Let's call $\alpha = \frac 15$ and $\beta = \frac 34$. On the $i$-th level all the nodes contains $\alpha^j \beta^{i-j}$; the number of nodes on the $i$-th level having $\alpha^j \beta^{i-j}$ elements to deal with is the number of possible way in which we can select $j$ left moves over $i$ total moves: so $\binom i j$ moves in total. Thus at each level $i$ we have
     $$
     \sum_{j=0}^i \binom i j \alpha^j \beta^{i-j} n
     \nonumber
     $$
     So this is the total number of elements we need to deal with at the $i$-th level of our recursion tree. We have that
     $$
     \sum_{j=0}^i \binom i j \alpha^j \beta^{i-j} n = (\alpha + \beta)^i \cdot n
     \nonumber
     $$
     To do an over approximation of the complexity, let's suppose that the tree has infinite length. So
     $$
     T(n) \le \sum_{i=0}^\infty (\alpha + \beta)^i \cdot n = \sum_{i=0}^\infty \left(\frac 15 + \frac 34 \right)^i \cdot n = \sum_{i=0}^\infty \left(\frac {19}{20} \right)^i \cdot n.
     \nonumber
     $$
     Because of the convergence of geometric series $\left( \frac{19}{20} < 1 \right)$ $T(n) \le \frac 1{1-\frac{19}{20}}n = 20n$, so $T(n) \in O(n)$.
   
     Can we lower bound it? Of course yes, since just the first call of our recursive call costs $\Theta(n)$, so $T(n) \in \Omega(n)$. Thus $T(n) \in \Theta(n)$.
   
     So just solving this problem we proved a new theorem:
   
     > **Theorem:** Let $\alpha$ and $\beta$ be two natural numbers. If $\alpha + \beta < 1$, then $T(n) = T(\alpha n) + T(\beta n) + \Theta(n)$ belongs to $\Theta(n)$.
   
   - $T_3(n) = 3 * T_3(n/2) + O(n)$
   
     Using the **recursion tree**, we have that, choosing $cn$ as representative for $O(n)$:
     $$
     \begin{align*}
     T_3(n) &= 3 * T_3(n/2) + O(n) \\
     &\le 3 * T_3(n/2) + cn \\
     &\le 3 * (3 * T_3(n/4) + cn/2) + cn \\
     &= 9 * T_3(n/4) + 3/2 cn + cn \\
     &= 9 * T_3(n/4) + 3/2 cn + cn \\
     &\le 9 * (3 * T_3(n/8) + cn/4) + 3/2 cn + cn \\
     &= 27 * T_3(n/8) + 9/4 cn + 3/2 cn + cn \\
     &\le 27* (3 * T_3(n/16) + cn/8) + 9/4 cn + 3/2 cn + cn \\
     &= 81 * T_3(n/16) + 27/8 cn + 9/4 cn + 3/2 cn + cn \\
     &\le \ldots \\
     &\le 3^{\log_2 n} \cdot T_3(0) + \sum_{i=0}^{\log_2 n} \left(\frac32\right)^i \cdot cn \\
     &= 0 + cn \cdot \frac{(3/2)^{(\log_2 n)+1} - 1}{3/2-1}
     = cn \cdot \frac{\frac{3^{(\log_2 n)+1} - 2^{(\log_2 n)+1}}{2^{(\log_2 n)+1}}}{\frac{3 - 2}{2}} \\
     &= 2cn \cdot \frac{3 \cdot 3^{\log_2 3 \cdot \log_3 n} - 2n}{2n}
     = c (3 \cdot (3^{\log_3 n})^{\log_2 3} - 2n) \\
     &= c (3 \cdot n^{\log_2 3} - 2n)
     = 3cn^{\log_2 3} - 2cn \in O(n^{\log_2 3})
     \end{align*}
     $$
     because since $\log_b n = \log_b a \cdot \log_a n$ we have that $\log_2 n = \log_2 3 \cdot \log_3 n$.
   
     Or directly
     $$
     \begin{align*}
     T_3(n) &= 3 * T_3(n/2) + O(n)  \le \sum_{i=0}^{\log_2 n} 3^i c \frac n{2^i} = cn \sum_{i=0}^{\log_2 n} \left(\frac32\right)^i = cn \cdot \frac{(3/2)^{(\log_2 n)+1}-1}{3/2 - 1} \\
     &= cn \cdot \frac{\frac{3^{(\log_2 n)+1} - 2^{(\log_2 n)+1}}{2^{(\log_2 n)+1}}}{\frac{3 - 2}{2}} = 2cn \cdot \frac{3 \cdot 3^{\log_2 3 \cdot \log_3 n} - 2n}{2n} = c (3 \cdot (3^{\log_3 n})^{\log_2 3} - 2n) \\
     &= c (3 \cdot n^{\log_2 3} - 2n) = 3cn^{\log_2 3} - 2cn \in O(n^{\log_2 3})
     \end{align*}
     $$
     Using the **substitution method**, we guess that $T_3 \in O(n^{\log_2 3})$ and we select the function $cn^{\log_2 3} - dn$ as representative, and we select $c'n$ as representative of $O(n)$. Inductive assumption: we assume that $\forall m < n, \; T_3(m) \le cm^{\log_2 3} - dm$. We want to prove that $\forall n, \; T_3(n) \le cn^{\log_2 3} - dn$. If this is the case we have that
     $$
     \begin{align*}
     T_3(n) &= 3 * T_3(n/2) + O(n) \\
     &\le 3 \left( c \left(\frac n2\right)^{\log_2 3} - d \frac n2 \right) + c'n \\
     &= 3 c \frac{n^{\log_2 3}}{2^{\log_2 3}} - n \left( \frac 32 d - c' \right) \\
     &= 3 c \frac{n^{\log_2 3}}3 - n \left(\frac{3d - 2c'}2 \right) \\
     &= c n^{\log_2 3} - \frac{3d - 2c'}2 n \\
     \end{align*}
     $$
     if $\frac{3d - 2c'}2 \le d \Longleftrightarrow 3d - 2c'\le 2d \Longleftrightarrow d \le 2c'$, then $T_3(n) \le c n^{\log_2 3} - dn$. Thus we have proved by induction that $\forall n \in \mathbb{N}, \; T_3(n) \le c n^{\log_2 3} - dn$ for a proper $c$ and $d$. So $T_3(n) \in O(n^{\log_2 3})$.
   
   - $T_4(n) = 7 * T_4(n/2) + \Theta(n^2)$
   
     Using the **recursion tree**, we have that, choosing $cn^2$ as representative for $\Theta(n^2)$:
     $$
     \begin{align*}
     T_4(n) &= 7 * T_4(n/2) + \Theta(n^2)\\
     &= 7 * T_4(n/2) + cn^2 \\
     &= 7 * \left(7 * T_4\left(\frac n4\right) + c\left(\frac n2\right)^2 \right) + cn^2 \\
     &= 49 * T_4\left(\frac n4 \right) + 7c\left(\frac n2\right)^2 + cn^2 \\
     &= 49 * \left(7 * T_4\left(\frac n8\right) + c\left(\frac n4\right)^2 \right) + 7c\left(\frac n2\right)^2 + cn^2 \\
     &= 343 * T_4\left(\frac n8\right) + 49c\left(\frac n4\right)^2 + 7c\left(\frac n2\right)^2 + cn^2 \\
     &= \ldots \\
     &= 7^{\log_2 n} T_4(0) + \sum_{i=0}^{\log_2 n} 7^i \cdot c \left(\frac n{2^i}\right)^2 \\
     &= 0 + cn^2 \sum_{i=0}^{\log_2 n} \left( \frac74 \right)^i
     = cn^2 \cdot \frac{(7/4)^{(\log_2 n)+1}-1}{7/4 - 1} \\
     &= cn^2 \cdot \frac{\frac{7^{(\log_2 n)+1} - 4^{(\log_2 n)+1}}{4^{(\log_2 n)+1}}}{\frac{7 - 4}{4}}
     = \frac43 cn^2 \cdot \frac{7 \cdot 7^{\log_2 7 \cdot \log_7 n} - 4\cdot4^{\log_2 n}}{4\cdot4^{\log_2 n}} \\
     &= \frac43 cn^2 \cdot \frac{7 \cdot (7^{\log_7 n})^{\log_2 7} - 4\cdot(2^{\log_2 n})^2}{4\cdot(2^{\log_2 n})^2}
     = \frac43 cn^2 \cdot \frac{7 \cdot n^{\log_2 7} - 4n^2}{4n^2} \\
     &= \frac73 c n^{\log_2 7} - \frac43 cn^2 \in O(n^{\log_2 7})
     \end{align*}
     $$
     Or directly
     $$
     \begin{align*}
     T_4(n) &= 7 * T_4(n/2) + \Theta(n^2) \le \sum_{i=0}^{\log_2 n} 7^i c \left(\frac n{2^i}\right)^2
     = cn^2 \sum_{i=0}^{\log_2 n} \left( \frac74 \right)^i
     = cn^2 \cdot \frac{(7/4)^{(\log_2 n)+1}-1}{7/4 - 1} \\
     &= cn^2 \cdot \frac{\frac{7^{(\log_2 n)+1} - 4^{(\log_2 n)+1}}{4^{(\log_2 n)+1}}}{\frac{7 - 4}{4}}
     = \frac43 cn^2 \cdot \frac{7 \cdot 7^{\log_2 7 \cdot \log_7 n} - 4\cdot4^{\log_2 n}}{4\cdot4^{\log_2 n}} \\
     &= \frac43 cn^2 \cdot \frac{7 \cdot (7^{\log_7 n})^{\log_2 7} - 4\cdot(2^{\log_2 n})^2}{4\cdot(2^{\log_2 n})^2}
     = \frac43 cn^2 \cdot \frac{7 \cdot n^{\log_2 7} - 4n^2}{4n^2} \\
     &= \frac73 c n^{\log_2 7} - \frac43 cn^2 \in O(n^{\log_2 7})
     \end{align*}
     $$
     Besides, we have that
     $$
     \begin{align*}
     T_4(n) &= 7 * T_4(n/2) + \Theta(n^2) \ge \sum_{i=0}^{\log_2 n} 7^i c \left(\frac n{2^i}\right)^2
     = cn^2 \sum_{i=0}^{\log_2 n} \left( \frac74 \right)^i
     = cn^2 \cdot \frac{(7/4)^{(\log_2 n)+1}-1}{7/4 - 1} \\
     &= cn^2 \cdot \frac{\frac{7^{(\log_2 n)+1} - 4^{(\log_2 n)+1}}{4^{(\log_2 n)+1}}}{\frac{7 - 4}{4}}
     = \frac43 cn^2 \cdot \frac{7 \cdot 7^{\log_2 7 \cdot \log_7 n} - 4\cdot4^{\log_2 n}}{4\cdot4^{\log_2 n}} \\
     &= \frac43 cn^2 \cdot \frac{7 \cdot (7^{\log_7 n})^{\log_2 7} - 4\cdot(2^{\log_2 n})^2}{4\cdot(2^{\log_2 n})^2}
     = \frac43 cn^2 \cdot \frac{7 \cdot n^{\log_2 7} - 4n^2}{4n^2} \\
     &= \frac73 c n^{\log_2 7} - \frac43 cn^2 \in \Omega(n^{\log_2 7})
     \end{align*}
     $$
     So we have that $T_4(n) \in \Theta(n^{\log_2 7})$.
   
     Using the **substitution method**, we guess that $T_4 \in O(n^{\log_2 7})$ and we select the function $cn^{\log_2 7} - dn^2$ as representative, and we select $c'n^2$ as representative of $\Theta(n^2)$. Inductive assumption: we assume that $\forall m < n, \; T_3(m) \le cm^{\log_2 7} - dm^2$. We want to prove that $\forall n, \; T_4(n) \le cn^{\log_2 7} - dn^2$. If this is the case we have that
     $$
     \begin{align*}
     T_4(n) &= 7 * T_4(n/2) + \Theta(n^2) \\
     &\le 7 \left( c \left(\frac n2\right)^{\log_2 7} - d \left(\frac n2\right)^2 \right) + c'n^2 \\
     &= 7 c \frac{n^{\log_2 7}}{2^{\log_2 7}} - 7d \frac{n^2}4 + c'n^2 \\
     &= 7 c \frac{n^{\log_2 7}}7 - n^2 \left(\frac74 d - c' \right) \\
     &= c n^{\log_2 7} - \frac{7d - 4c'}4 n^2 \\
     \end{align*}
     $$
     if $\frac{7d - 4c'}4 \le d \Longleftrightarrow 7d - 4c'\le 4d \Longleftrightarrow 3d \le 4c' \Longleftrightarrow d \le \frac43 c'$, then $T_4(n) \le c n^{\log_2 7} - dn^2$. Thus we have proved by induction that $\forall n \in \mathbb{N}, \; T_3(n) \le c n^{\log_2 7} - dn^2$ for a proper $c$ and $d$. So $T_3(n) \in O(n^{\log_2 7})$.
   
     Now we want to prove that $T_4(n) \in \Omega(n^{\log_2 7})$. We select the representative $cn^{\log_2 7} \in \Omega(n^{\log_2 7})$ and the representative $c'n^2 \in \Theta(n^2)$. Inductive assumption: we assume that $\forall m < n, \; T_4(m) \ge cm^{\log_2 7}$. We want to prove that $\forall n, \; T_4(n) \ge cn^{\log_2 7}$.
     $$
     \begin{align*}
     T_4(n) &= 7 * T_4(n/2) + \Theta(n^2) \\
     &\ge 7 c \left(\frac n2\right)^{\log_2 7}+ c'n^2 \\
     &= 7 c \frac{n^{\log_2 7}}{2^{\log_2 7}} + c'n^2 \\
     &=  7 c \frac{n^{\log_2 7}}{7} + c'n^2 \\
     &= c n^{\log_2 7} + c'n^2 \\
     &\ge c n^{\log_2 7}
     \end{align*}
     $$
     Thus we have that $T_4(n) \ge cn^{\log_2 7}$, so we have proved by induction that $\forall n \in \mathbb{N}, \; T_3(n) \ge c n^{\log_2 7} - dn^2$ for a proper $c$. Then $T_4(n) \in \Omega(n^{\log_2 7})$. Therefore we have proved that $T_4(n) \in \Theta(n^{\log_2 7})$.



### References

<a name="ref1"></a> [1] T.H. Cormen, C.E. Leiserson, R.L. Rivest, and C. Stein. *Introduction to Algorithms*. The MIT Press. MIT Press, 2009.